Add missing examples and annotations to grind annotations section

Manual/Grind/Annotation.lean
@@ -17,61 +17,127 @@ open Verso.Doc.Elab (CodeBlockExpander)
 
 open Lean.Elab.Tactic.GuardMsgs.WhitespaceMode
 
-#doc (Manual) "Annotating libraries for `grind`" =>
+#doc (Manual) "Annotating Libraries for `grind`" =>
 %%%
-tag := "grind annotation"
+tag := "grind-annotation"
 %%%
 
-(work-in-progress, this needs examples)
+To use {tactic}`grind` effectively with a library, it must be annotated by applying the {attr}`grind` attribute to suitable lemmas or declaring {keywordOf Lean.Parser.Command.grindPattern}`grind_pattern`s.
+These annotations direct {tactic}`grind`'s selection of theorems, which lead to further facts on the metaphorical whiteboard.
+With too few annotations, {tactic}`grind` will fail to use the lemmas; with too many, it may become slow or it fail due to exhausting resource limitations.
+Annotations should generally be conservative: only add an annotation if you expect that {tactic}`grind` should _always_ instantiate the theorem once the patterns are matched.
 
-Annotations should generally be conservative: only add an attribute or grind pattern when
-you expect that {tactic}`grind` should always instantiate the theorem once the patterns are matched.
+# Simp Lemmas
 
-Typically, many theorems that are annotated with `@[simp]` will also be need to be annotated with `@[grind =]`.
-One significant exception is that typically we avoid having `@[simp]` theorems that introduce an `if` on the right hand side,
-instead preferring a pair of theorems with the positive and negative conditions as hypotheses.
-Because `grind` is designed to perform case splitting, it is generally better to instead label the single theorem introducing the `if` with `@[grind =]`.
+Typically, many theorems that are annotated with {attrs}`@[simp]` should also be annotated with {attrs}`@[grind =]`.
+One significant exception is that typically we avoid having {attrs}`@[simp]` theorems that introduce an {keywordOf Lean.Parser.Term.if}`if` on the right hand side, instead preferring a pair of theorems with the positive and negative conditions as hypotheses.
+Because {tactic}`grind` is designed to perform case splitting, it is generally better to instead annotate the single theorem introducing the {keywordOf Lean.Parser.Term.if}`if` with {attrs}`@[grind =]`.
 
-Besides using `@[grind =]` to encourage {tactic}`grind` to perform rewriting from left to right,
-you can also use `@[grind _=_]` to "saturate", allowing bidirectional rewriting whenever either side is encountered.
+Besides using {attrs}`@[grind =]` to encourage {tactic}`grind` to perform rewriting from left to right, you can also use {attrs}`@[grind _=_]` to “saturate”, allowing bidirectional rewriting whenever either side is encountered.
 
-Use `@[grind ←]` (which generates patterns from the conclusion of the theorem) for backwards reasoning theorems,
-i.e. theorems that should be tried when their conclusion matches a goal.
+# Backwards and Forwards Reasoning
 
-Use `@[grind →]` (which generates patterns from the hypotheses) for forwards reasoning theorems,
+:::paragraph
+Use {attrs}`@[grind ←]` (which generates patterns from the conclusion of the theorem) for backwards reasoning theorems, i.e. theorems that should be tried when their conclusion matches a goal.
+Some examples of theorems in the standard library that are annotated with {attr}`grind ←` are:
+* ```signature
+  Array.not_mem_empty (a : α) : ¬ a ∈ #[]
+  ```
+* ```signature
+  Array.getElem_filter {xs : Array α} {p : α → Bool} {i : Nat} (h : i < (xs.filter p).size) :
+    p (xs.filter p)[i]
+  ```
+* ```signature
+  List.Pairwise.tail : ∀ {l : List α} (h : Pairwise R l), Pairwise R l.tail
+  ```
+In each case, the lemma is relevant when its conclusion matches a proof goal.
+:::
+
+:::paragraph
+Use {attrs}`@[grind →]` (which generates patterns from the hypotheses) for forwards reasoning theorems,
 i.e. where facts should be propagated from existing facts on the whiteboard.
+Some examples of theorems in the standard library that are annotated with {attr}`grind →` are:
+* ```signature
+  List.getElem_of_getElem? {l : List α} : l[i]? = some a → ∃ h : i < l.length, l[i] = a
+  ```
+* ```signature
+  Array.mem_of_mem_erase [BEq α] {a b : α} {xs : Array α} (h : a ∈ xs.erase b) : a ∈ xs
+  ```
+* ```signature
+  List.forall_none_of_filterMap_eq_nil (h : filterMap f xs = []) : ∀ x ∈ xs, f x = none
+  ```
+In these cases, the theorems' assumptions determine when they are relevant.
+:::
 
-There are many uses for custom patterns created with the `grind_pattern` command.
+There are many uses for custom patterns created with the {keywordOf Lean.Parser.Command.grindPattern}`grind_pattern` command.
 One common use is to introduce inequalities about terms, or membership propositions.
 
-We might have
+:::keepEnv
+```lean -show
+section
+def count := @Array.count
+theorem countP_le_size [BEq α] {a : α} {xs : Array α} : count a xs ≤ xs.size := Array.countP_le_size
+notation "..." => countP_le_size
 ```
-theorem count_le_size {a : α} {xs : Array α} : count a xs ≤ xs.size := countP_le_size
+
+We might have
+```lean
+variable [BEq α]
+
+theorem count_le_size {a : α} {xs : Array α} : count a xs ≤ xs.size :=
+  ...
 
 grind_pattern count_le_size => count a xs
 ```
-which will register this inequality as soon as a `count a xs` term is encountered (even if the problem has not previously involved inequalities).
-
-We can also use multi-patterns to be more restrictive,
-e.g. only introducing an inequality about sizes if the whiteboard already contains facts about sizes:
+```lean -show
+variable {a : α} {xs : Array α}
 ```
-theorem size_pos_of_mem {a : α} {xs : Array α} (h : a ∈ xs) : 0 < xs.size := sorry
+which will register this inequality as soon as a {lean}`count a xs` term is encountered (even if the problem has not previously involved inequalities).
+
+```lean -show
+end
+```
+:::
+
+We can also use multi-patterns to be more restrictive, e.g. only introducing an inequality about sizes if the whiteboard already contains facts about sizes:
+```lean
+theorem size_pos_of_mem {xs : Array α} (h : a ∈ xs) : 0 < xs.size :=
+  sorry
 
 grind_pattern size_pos_of_mem => a ∈ xs, xs.size
 ```
-Unlike `@[grind →]` attribute, which would cause this theorem to be instantiated whenever `a ∈ xs` is encountered,
-this pattern will only be used when `xs.size` is already on the whiteboard.
-(Note that this grind pattern could also be produced using the `@[grind <=]` attribute, which looks at the conclusion first,
-then backwards through the hypotheses to select patterns. On the other hand `@[grind →]` would select only `a ∈ xs`.)
+:::leanSection
+```lean -show
+variable {a : α} {xs : Array α}
+```
+Unlike a {attrs}`@[grind →]` attribute, which would cause this theorem to be instantiated whenever {lean}`a ∈ xs` is encountered, this pattern will only be used when {lean}`xs.size` is already on the whiteboard.
+(Note that this grind pattern could also be produced using the {attrs}`@[grind <=]` attribute, which looks at the conclusion first, then backwards through the hypotheses to select patterns.
+On the other hand, {attrs}`@[grind →]` would select only {lean}`a ∈ xs`.)
+:::
 
+
+::::keepEnv
+:::leanSection
+```lean -show
+axiom R : Type
+axiom sin : R → R
+axiom cos : R → R
+@[instance] axiom instAdd : Add R
+@[instance] axiom instOfNatR : OfNat R n
+@[instance] axiom instHPowR : HPow R Nat R
+variable {x : R}
+axiom sin_sq_add_cos_sq' : sin x ^ 2 + cos x ^ 2 = 1
+notation "..." => sin_sq_add_cos_sq'
+```
 In Mathlib we might want to enable polynomial reasoning about the sine and cosine functions,
 and so add a custom grind pattern
-```
+```lean
 theorem sin_sq_add_cos_sq : sin x ^ 2 + cos x ^ 2 = 1 := ...
 
 grind_pattern sin_sq_add_cos_sq => sin x, cos x
 ```
-which will instantiate the theorem as soon as *both* `sin x` and `cos x` (with the same `x`) are encountered.
-This theorem will then automatically enter the Gröbner basis module,
-and be used to reason about polynomial expressions involving both `sin x` and `cos x`.
-One both alternatively, more aggressively, write two separate grind patterns so that this theorem instantiated when either `sin x` or `cos x` is encountered.
+which will instantiate the theorem as soon as *both* {lean}`sin x` and {lean}`cos x` (with the same {lean}`x`) are encountered.
+This theorem will then automatically enter the Gröbner basis module, and be used to reason about polynomial expressions involving both {lean}`sin x` and {lean}`cos x`.
+One both alternatively, more aggressively, write two separate grind patterns so that this theorem instantiated when either {lean}`sin x` or {lean}`cos x` is encountered.
+:::
+::::
